proof_of_soundness/NoMacroInvocations.v
@@ -29,21 +29,21 @@ Inductive ExprNoMacroInvocations : expr -> function_table -> macro_table -> Prop
     ExprNoMacroInvocations (Assign x e0) F M
   | NM_CallOrInvocation : forall x es F M params fstmt fexpr,
     ~ StringMap.In x M ->
-    NoMacroInvocationsArgs es F M ->
+    ExprListNoMacroInvocations es F M ->
     StringMap.MapsTo x (params, fstmt, fexpr) F ->
     ExprNoMacroInvocations fexpr F M ->
     ExprNoMacroInvocations (CallOrInvocation x es) F M
-with NoMacroInvocationsArgs : list expr -> function_table -> macro_table -> Prop :=
-  | NM_Args_nil : forall F M,
-    NoMacroInvocationsArgs nil F M
-  | NM_Args_cons : forall e es F M,
+with ExprListNoMacroInvocations : list expr -> function_table -> macro_table -> Prop :=
+  | NM_ExprList_nil : forall F M,
+    ExprListNoMacroInvocations nil F M
+  | NM_ExprList_cons : forall e es F M,
     ExprNoMacroInvocations e F M ->
-    NoMacroInvocationsArgs es F M ->
-    NoMacroInvocationsArgs (e::es) F M.
+    ExprListNoMacroInvocations es F M ->
+    ExprListNoMacroInvocations (e::es) F M.
 
 
 Scheme ExprNoMacroInvocations_mut := Induction for ExprNoMacroInvocations Sort Prop
-with NoMacroInvocationsArgs_mut := Induction for NoMacroInvocationsArgs Sort Prop.
+with ExprListNoMacroInvocations_mut := Induction for ExprListNoMacroInvocations Sort Prop.
 
 
 Lemma ExprNoMacroInvocations_remove_ExprNoMacroInvocations : forall e F M,
@@ -55,9 +55,9 @@ Proof.
     (fun e F M (h : ExprNoMacroInvocations e F M) =>
       forall x,
       ExprNoMacroInvocations e F (StringMap.remove x M))
-    (fun es F M (h : NoMacroInvocationsArgs es F M) =>
+    (fun es F M (h : ExprListNoMacroInvocations es F M) =>
       forall x,
-      NoMacroInvocationsArgs es F (StringMap.remove x M))); try constructor; auto.
+      ExprListNoMacroInvocations es F (StringMap.remove x M))); try constructor; auto.
   - intros. econstructor; auto.
     + unfold not. intros. apply StringMapFacts.remove_in_iff in H1. destruct H1.
       contradiction.
@@ -65,7 +65,7 @@ Proof.
 Qed.
 
 
-Lemma ExprNoMacroInvocations_remove_EvalExpr : forall S E G F M e v S',
+Lemma EvalExprNoMacroInvocations_remove_EvalExpr : forall S E G F M e v S',
   EvalExpr S E G F M e v S' ->
   ExprNoMacroInvocations e F M ->
   forall x,
@@ -82,11 +82,11 @@ Proof.
       (fun S E G F M stmt S' (h : EvalStmt S E G F M stmt S' ) =>
         forall (x : string),
         EvalStmt S E G F (StringMap.remove x M) stmt S' (* TODO: Fix once more statement are added *))
-      (* EvalArgs *)
-      (fun Sprev Ecaller G F M ps es vs Snext Ef Sargs l (h : EvalArgs Sprev Ecaller G F M ps es vs Snext Ef Sargs l) =>
-        NoMacroInvocationsArgs es F M ->
+      (* EvalExprList *)
+      (fun Sprev Ecaller G F M ps es vs Snext Ef Sargs l ls (h : EvalExprList Sprev Ecaller G F M ps es vs Snext Ef Sargs l ls) =>
+        ExprListNoMacroInvocations es F M ->
         forall x,
-        EvalArgs Sprev Ecaller G F (StringMap.remove x M) ps es vs Snext Ef Sargs l )); auto; intros; try constructor.
+        EvalExprList Sprev Ecaller G F (StringMap.remove x M) ps es vs Snext Ef Sargs l ls)); auto; intros; try constructor.
   - apply E_LocalVar with l; auto.
   - apply E_GlobalVar with l; auto.
   - inversion_clear H0; auto.
@@ -95,7 +95,7 @@ Proof.
   - inversion_clear H0. apply E_Assign_Local with l S'; auto.
   - inversion_clear H0. apply E_Assign_Global with l S'; auto.
   - inversion_clear H2. apply E_FunctionCall with
-    params fstmt fexpr ls Ef Sargs S' S'' S''' S'''' vs l; auto.
+    params fstmt fexpr l ls Ef Sargs S' S'' S''' S'''' vs; auto.
     + unfold not. intros. apply StringMapFacts.remove_in_iff in H2.
       destruct H2. contradiction.
     + apply H1; auto.
@@ -107,14 +107,14 @@ Proof.
 Qed.
 
 
-Lemma ExprNoMacroInvocations_remove_EvalArgs : forall Sprev Ecaller G F M ps es vs Snext Ef Sargs l,
-  EvalArgs Sprev Ecaller G F M ps es vs Snext Ef Sargs l ->
-  NoMacroInvocationsArgs es F M ->
+Lemma ExprNoMacroInvocations_remove_EvalExprList : forall Sprev Ecaller G F M ps es vs Snext Ef Sargs l ls,
+  EvalExprList Sprev Ecaller G F M ps es vs Snext Ef Sargs l ls->
+  ExprListNoMacroInvocations es F M ->
   forall x,
-  EvalArgs Sprev Ecaller G F (StringMap.remove x M) ps es vs Snext Ef Sargs l.
+  EvalExprList Sprev Ecaller G F (StringMap.remove x M) ps es vs Snext Ef Sargs l ls.
 Proof.
   apply (
-    EvalArgs_mut
+    EvalExprList_mut
       (* EvalExpr *)
       (fun S E G F M e v S' (h : EvalExpr S E G F M e v S') =>
         ExprNoMacroInvocations e F M ->
@@ -124,11 +124,11 @@ Proof.
       (fun S E G F M stmt S' (h : EvalStmt S E G F M stmt S' ) =>
         forall (x : string),
         EvalStmt S E G F (StringMap.remove x M) stmt S' (* TODO: Fix once more statement are added *))
-      (* EvalArgs *)
-      (fun Sprev Ecaller G F M ps es vs Snext Ef Sargs l (h : EvalArgs Sprev Ecaller G F M ps es vs Snext Ef Sargs l) =>
-        NoMacroInvocationsArgs es F M ->
+      (* EvalExprList *)
+      (fun Sprev Ecaller G F M ps es vs Snext Ef Sargs l ls (h : EvalExprList Sprev Ecaller G F M ps es vs Snext Ef Sargs l ls) =>
+        ExprListNoMacroInvocations es F M ->
         forall x,
-        EvalArgs Sprev Ecaller G F (StringMap.remove x M) ps es vs Snext Ef Sargs l )); auto; intros; try constructor.
+        EvalExprList Sprev Ecaller G F (StringMap.remove x M) ps es vs Snext Ef Sargs l ls)); auto; intros; try constructor.
   - apply E_LocalVar with l; auto.
   - apply E_GlobalVar with l; auto.
   - inversion_clear H0; auto.
@@ -137,7 +137,7 @@ Proof.
   - inversion_clear H0. apply E_Assign_Local with l S'; auto.
   - inversion_clear H0. apply E_Assign_Global with l S'; auto.
   - inversion_clear H2. apply E_FunctionCall with
-    params fstmt fexpr ls Ef Sargs S' S'' S''' S'''' vs l; auto.
+    params fstmt fexpr l ls Ef Sargs S' S'' S''' S'''' vs; auto.
     + unfold not. intros. apply StringMapFacts.remove_in_iff in H2.
       destruct H2. contradiction.
     + apply H1; auto.
@@ -161,10 +161,10 @@ Proof.
       forall F',
       ExprNoCallsFromFunctionTable e F M F' ->
       ExprNoMacroInvocations e (StringMapProperties.update F F') M)
-    (fun es F M (h : NoMacroInvocationsArgs es F M) =>
+    (fun es F M (h : ExprListNoMacroInvocations es F M) =>
       forall F',
-      ExprNoCallsFromFunctionTableArgs es F M F' ->
-      NoMacroInvocationsArgs es (StringMapProperties.update F F') M)); intros; try constructor; auto.
+      ExprListNoCallsFromFunctionTable es F M F' ->
+      ExprListNoMacroInvocations es (StringMapProperties.update F F') M)); intros; try constructor; auto.
   - inversion_clear H0; auto.
   - inversion_clear H0; auto.
   - inversion_clear H1; auto.
@@ -179,6 +179,21 @@ Proof.
     + apply StringMap_mapsto_in in H4. contradiction.
   - inversion_clear H1; auto.
   - inversion_clear H1; auto.
+Qed.
+
+
+Lemma ExprListNoMacroInvocations_update_ExprNoCallsFromFunctionTableExprList_ExprListNoMacroInvocations:
+  forall es F M,
+  ExprListNoMacroInvocations es F M ->
+  forall F',
+  ExprListNoCallsFromFunctionTable es F M F' ->
+  ExprListNoMacroInvocations es (StringMapProperties.update F F') M.
+Proof.
+  intros. induction H0.
+  - constructor.
+  - inversion_clear H.
+    constructor; auto.
+    apply ExprNoMacroInvocations_update_ExprNoCallFromFunctionTable_ExprNoMacroInvocations; auto. 
 Qed.
 
 
@@ -218,12 +233,12 @@ Proof.
         forall p ef,
         MSub p e mexpr ef ->
         ExprNoMacroInvocations ef F M)
-    (fun es F M (h : NoMacroInvocationsArgs es F M) =>
+    (fun es F M (h : ExprListNoMacroInvocations es F M) =>
         forall e,
         ExprNoMacroInvocations e F M ->
         forall p es',
         MSubList p e es es' ->
-        NoMacroInvocationsArgs es' F M)); intros; try (inversion_clear H0; constructor; auto).
+        ExprListNoMacroInvocations es' F M)); intros; try (inversion_clear H0; constructor; auto).
   - inversion H0.
     + subst. auto.
     + subst. constructor.
@@ -236,17 +251,17 @@ Proof.
     + constructor. apply H with e1 p; auto.
     + constructor. apply H with e1 p; auto.
   - inversion_clear H2. apply NM_CallOrInvocation with params fstmt fexpr; auto.
-    apply H with e0 p; auto.
+    apply H with e1 p; auto.
   - inversion_clear H2. constructor.
-    + apply H with e1 p; auto.
-    + apply H0 with e1 p; auto.
+    + apply H with e2 p; auto.
+    + apply H0 with e2 p; auto.
 Qed.
 
 
-Lemma ExprNoMacroInvocations_NoMacroInvocationArgs_MacroSubst_ExprNoMacroInvocations : forall mexpr F M,
+Lemma ExprNoMacroInvocations_NoMacroInvocationExprList_MacroSubst_ExprNoMacroInvocations : forall mexpr F M,
   ExprNoMacroInvocations mexpr F M ->
   forall es,
-  NoMacroInvocationsArgs es F M ->
+  ExprListNoMacroInvocations es F M ->
   forall ps ef,
   MacroSubst ps es mexpr ef ->
   ExprNoMacroInvocations ef F M.
