proof_of_soundness/Transformations.v
@@ -20,16 +20,20 @@ Inductive TransformExpr :
   function_table -> expr -> Prop :=
 
   | Transform_Num : forall M F z,
+    (* Identity transformation *)
     TransformExpr M F (Num z) F (Num z)
 
   | Transform_Var : forall M F x,
+    (* Identity transformation *)
     TransformExpr M F (Var x) F (Var x)
 
   | Transform_ParenExpr : forall M F e0 F' e0',
+    (* Transform the inner expression *)
     TransformExpr M F e0 F' e0' ->
     TransformExpr M F (ParenExpr e0) F' (ParenExpr e0')
 
   | Transform_UnExpr : forall M F e0 F' e0' uo,
+    (* Transform the inner expression *)
     TransformExpr M F e0 F' e0' ->
     TransformExpr M F (UnExpr uo e0) F' (UnExpr uo e0')
 
@@ -43,27 +47,24 @@ Inductive TransformExpr :
     TransformExpr M F' e2 F'' e2' ->
     F'' = StringMapProperties.update F' F2result ->
 
-    (* None of the function calls in e1 are to functions that were added
+    (* What I find interesting here is what we *don't* need to add
+       as premises in order for the proof to work *)
+
+    (* e1 does not contain calls are to functions that were added
        while transforming e2 *)
-    ExprNoCallsFromFunctionTable e1 F M F2result ->
-    (* None of the functions calls in e1' are to functions that were added
+    (* ExprNoCallsFromFunctionTable e1 F M F2result -> *)
+
+    (* e1' does not contain calls to functions that were added
        while transforming e2 *)
     ExprNoCallsFromFunctionTable e1' F' M F2result ->
-    (* None of the functions calls in e2 are to functions that were added
+
+    (* e2 does not contain calls to functions that were added
        while transforming e1 *)
     ExprNoCallsFromFunctionTable e2 F M F1result ->
-    (* None of the functions calls in e2' are to functions that were added
-       while transforming e1 *)
-    ExprNoCallsFromFunctionTable e2' F'' M F1result ->
 
-    (* This is interesting - In order for the proof to succeed, we must assert that
-     both the left and right transformations result in ultimately the same function
-     table. This is what we do in our unification step.
-     This looks funny, but it makes sense when we consider the fact that our
-     transformation is defined in "big-step" notation - that is, we are not concerned
-     with the intermediate results, just that the final function table between these
-     two operands should be equal. If we were to define the semantics using small-step
-     notation, then we would have to transform each operand one at a time *)
+    (* e2' does not contain calls to functions that were added
+       while transforming e1 *)
+    (* ExprNoCallsFromFunctionTable e2' F'' M F1result -> *)
 
     TransformExpr M F (BinExpr bo e1 e2) F'' (BinExpr bo e1' e2')
 
@@ -72,64 +73,130 @@ Inductive TransformExpr :
     TransformExpr M F (Assign x e) F' (Assign x e')
 
   | Transform_FunctionCall :
-    forall   F M x es F' es'
-             params fstmt fexpr fstmt' fexpr',
+    forall   F M x es F' F'' F''' F'''' es' newdef
+             params fstmt fexpr fstmt' fexpr'
+             Fesresult Fstmtresult Fexprresult,
 
     ~ StringMap.In x M ->
     StringMap.MapsTo x (params, fstmt, fexpr) F ->
 
     (* Transform function arguments *)
-    TransformArgs M F es F' es' ->
+    TransformExprList M F es F' es' ->
+    F' = StringMapProperties.update F Fesresult ->
 
     (* Transform function statement *)
-    TransformStmt M F fstmt F' fstmt' ->
+    TransformStmt M F' fstmt F'' fstmt' ->
+    F'' = StringMapProperties.update F' Fstmtresult ->
 
     (* Transform function return expression *)
-    TransformExpr M F fexpr F' fexpr' ->
+    TransformExpr M F'' fexpr F''' fexpr' ->
+    F''' =  StringMapProperties.update F'' Fexprresult ->
+
+    (* Create the new definition of the function *)
+    newdef = (params, fstmt', fexpr') ->
+
+    (* es' does not contain calls to functions that
+       were added while transforming fstmt or fexpr or
+       the transformed function *)
+    ExprListNoCallsFromFunctionTable es' F' M Fstmtresult ->
+    ExprListNoCallsFromFunctionTable es' F'' M Fexprresult ->
+    ExprListFunctionNotCalled es' F''' M x newdef ->
+
+    (* fstmt' does not contain calls to functions that
+       were added while transforming fexpr or the transformed function *)
+    StmtNoCallsFromFunctionTable fstmt' F'' M Fexprresult ->
+    StmtFunctionNotCalled fstmt' F''' M x newdef ->
+
+    (* fexpr' does not contain a call to the transformed function or
+       to functions that were added while transforming fstmt *)
+    ExprFunctionNotCalled fexpr' F''' M x newdef ->
+
+    (* fexpr does not contain calls to functions that were added
+       while transforming fstmt or es *)
+    ExprNoCallsFromFunctionTable fexpr F M Fstmtresult ->
+    ExprNoCallsFromFunctionTable fexpr F' M Fstmtresult ->
+    ExprNoCallsFromFunctionTable fexpr F M Fesresult ->
+
+    (* fstmt does not contain calls to functions that were added
+       while transforming es *)
+    StmtNoCallsFromFunctionTable fstmt F M Fesresult ->
 
     (* Add the transformed function back to the function table under a new name *)
-    F' = StringMap.add x (params, fstmt', fexpr') F ->
+    F'''' = StringMapProperties.update F'''
+      (StringMap.add x newdef (StringMap.empty function_definition)) ->
 
-    TransformExpr M F (CallOrInvocation x es) F' (CallOrInvocation x es')
+    TransformExpr M F (CallOrInvocation x es) F'''' (CallOrInvocation x es')
+
+
+  | Transform_MacroIdentity :
+    forall F M x es params mexpr,
+
+    (* TODO: Decide if we should recursively transform macros if one part
+       of them makes the unable to be transformed.
+       For now we don't transform them at all. *)
+
+    StringMap.MapsTo x (params, mexpr) M ->
+
+    (* We don't transform the macro if:
+       - One of its arguments has side-effects
+       - Its body has side-effects
+       - Its body shares variables with its caller's environment
+    *)
+    Exists ExprHasSideEffects es \/
+    ExprHasSideEffects mexpr \/
+    (forall S E G v S',
+      EvalExpr S E G F M (CallOrInvocation x nil) v S' ->
+      ~ ExprNoVarsInEnvironment mexpr E) ->
+
+    TransformExpr M F (CallOrInvocation x es) F (CallOrInvocation x es)
 
   | Transform_ObjectLikeMacroNoSideEffectsNoSharedVarsNoNestedMacros :
-    forall F M x F' params mexpr mexpr' fname,
+    forall F M x F' params mexpr mexpr' fname newdef,
+
     StringMap.MapsTo x (params, mexpr) M ->
 
     (* The macro does not have side-effects *)
     ~ ExprHasSideEffects mexpr ->
     (* The macro does not contain nested macro invocations *)
     ExprNoMacroInvocations mexpr F M ->
-    (* The macro does not share variables with the caller environment *)
+
+    (* The macro does not share variables with its caller's environment *)
     (forall S E G v S',
       EvalExpr S E G F M (CallOrInvocation x nil) v S' ->
       ExprNoVarsInEnvironment mexpr E) ->
+
     (* Transform macro body *)
     TransformExpr M F mexpr F' mexpr' ->
+
+    (* Create the transformed definition *)
+    newdef = (nil, Skip, mexpr') ->
+
+    (* mexpr' does not contain a call to the transformed function *)
+    ExprFunctionNotCalled mexpr' F' M x newdef ->
 
     (* Add the transformed function definition to the function table *)
     ~ StringMap.In fname M ->
     ~ StringMap.In fname F ->
-    F' = StringMap.add fname (nil, Skip, mexpr') F ->
+    F' = StringMap.add fname newdef F ->
 
     TransformExpr M F (CallOrInvocation x nil) F' (CallOrInvocation fname nil)
-with TransformArgs :
+with TransformExprList :
   macro_table -> function_table -> list expr ->
   function_table -> list expr -> Prop :=
 
   (* End of arguments *)
-  | TransformArgs_Nil : forall M F,
-    TransformArgs M F nil F nil
+  | TransformExprList_Nil : forall M F,
+    TransformExprList M F nil F nil
 
   (* There are arguments left to transform *)
-  | TransformArgs_Cons : forall M F e es F' e' es',
+  | TransformExprList_Cons : forall M F e es F' e' es',
     (* Transform the first expression *)
     TransformExpr M F e F' e' ->
 
     (* Transform the remaining expressions *)
-    TransformArgs M F es F' es' ->
+    TransformExprList M F es F' es' ->
 
-    TransformArgs M F (e::es) F' (e'::es')
+    TransformExprList M F (e::es) F' (e'::es')
 with TransformStmt :
   macro_table -> function_table -> stmt ->
   function_table -> stmt -> Prop :=
@@ -139,7 +206,7 @@ with TransformStmt :
 
 
 Scheme TransformExpr_mut := Induction for TransformExpr Sort Prop
-with TransformArgs_mut := Induction for TransformArgs Sort Prop
+with TransformExprList_mut := Induction for TransformExprList Sort Prop
 with TransformStmt_mut := Induction for TransformStmt Sort Prop.
 
 
@@ -160,29 +227,31 @@ Lemma not_ExprHasSideEffects_TransformExpr_not_ExprHasSideEffects : forall e,
     ~ ExprHasSideEffects e'.
 Proof.
   intros. induction H0; auto.
-  -
+  - (* BinExpr *)
     simpl in H. apply Classical_Prop.not_or_and in H. destruct H.
     unfold ExprHasSideEffects. fold ExprHasSideEffects.
     apply Classical_Prop.and_not_or. split; auto.
 Qed.
 
 
-Lemma not_ExprHasSideEffects_TransformArgs_Forall_not_ExprHasSideEffects : forall es,
+Lemma not_ExprHasSideEffects_TransformExprList_Forall_not_ExprHasSideEffects : forall es,
   Forall (fun e => ~ ExprHasSideEffects e) es ->
   forall M F F' es',
-    TransformArgs M F es F' es' ->
+    TransformExprList M F es F' es' ->
   Forall (fun e => ~ ExprHasSideEffects e) es'.
 Proof.
   intros. induction H0.
-  - auto.
-  - inversion H. subst. apply Forall_cons.
-    * apply not_ExprHasSideEffects_TransformExpr_not_ExprHasSideEffects with e M F F'; auto.
-    * apply IHTransformArgs; auto.
+  - (* nil *)
+    auto.
+  - (* cons *)
+    inversion H. subst. constructor; auto.
+    (* Prove the head of the list doesn't have side-effects *)
+    apply not_ExprHasSideEffects_TransformExpr_not_ExprHasSideEffects with e M F F'; auto.
 Qed.
 
 
 (* This proof is easy right now because we only have Skip statements *)
-Lemma EvalStmt_TransformArgs_EvalStmt : forall S E G F M stmt S' F' stmt',
+Lemma EvalStmt_TransformExprList_EvalStmt : forall S E G F M stmt S' F' stmt',
   EvalStmt S E G F M stmt S' ->
   TransformStmt M F stmt F' stmt' ->
   EvalStmt S E G F' M stmt S'.
@@ -201,30 +270,30 @@ Proof.
     (fun M F e F' e' (h : TransformExpr M F e F' e') =>
       ExprNoMacroInvocations e F M ->
       e = e')
-    (* TransformArgs *)
-    (fun M F es F' es' (h : TransformArgs M F es F' es') =>
-      NoMacroInvocationsArgs es F M ->
+    (* TransformExprList *)
+    (fun M F es F' es' (h : TransformExprList M F es F' es') =>
+      ExprListNoMacroInvocations es F M ->
       es = es')
     (* TransformStmt *)
     (fun M F stmt F' stmt' (h : TransformStmt M F stmt F' stmt') =>
       True (* TODO: Fix this later once we add more statements *))); intros; auto.
-  -
+  - (* ParenExpr *)
     f_equal. inversion_clear H0; auto.
-  -
+  - (* UnExpr *)
     f_equal. inversion_clear H0; auto.
-  -
+  - (* BinExpr *)
     inversion_clear H1.
     f_equal; auto.
     apply H0. subst F'.
     apply ExprNoMacroInvocations_update_ExprNoCallFromFunctionTable_ExprNoMacroInvocations;
       auto.
-  -
+  - (* Assign *)
     inversion_clear H0. f_equal; auto.
-  -
+  - (* Function call *)
     inversion_clear H2. f_equal; auto.
-  -
+  - (* Macro invocation (contradiction) *)
     inversion_clear H0.  apply StringMap_mapsto_in in m. contradiction.
-  -
+  - (* ExprList *)
     inversion_clear H1. f_equal; auto.
 Qed.
 
@@ -239,16 +308,19 @@ Proof.
     (fun M F e F' e' (h : TransformExpr M F e F' e') =>
       ExprNoMacroInvocations e F M ->
       ExprNoMacroInvocations e' F' M)
-    (* TransformArgs *)
-    (fun M F es F' es' (h : TransformArgs M F es F' es') =>
-      NoMacroInvocationsArgs es F M ->
-      NoMacroInvocationsArgs es' F' M)
+    (* TransformExprList *)
+    (fun M F es F' es' (h : TransformExprList M F es F' es') =>
+      ExprListNoMacroInvocations es F M ->
+      ExprListNoMacroInvocations es' F' M)
     (* TransformStmt *)
     (fun M F stmt F' stmt' (h : TransformStmt M F stmt F' stmt') =>
       True (* TODO: Fix this later once we add more statements *))); intros; auto.
-  - inversion_clear H0. constructor; auto.
-  - inversion_clear H0. constructor; auto.
-  - inversion_clear H1. constructor; auto.
+  - (* ParenExpr *)
+    inversion_clear H0. constructor; auto.
+  - (* UnExpr *)
+    inversion_clear H0. constructor; auto.
+  - (* BinExpr *)
+    inversion_clear H1. constructor; auto.
     + subst F''.
       apply ExprNoMacroInvocations_update_ExprNoCallFromFunctionTable_ExprNoMacroInvocations;
         auto.
@@ -256,65 +328,56 @@ Proof.
       subst F'.
       apply ExprNoMacroInvocations_update_ExprNoCallFromFunctionTable_ExprNoMacroInvocations;
         auto.
-  - inversion_clear H0. constructor; auto.
-  - inversion_clear H2. 
+  - (* Assign *)
+    inversion_clear H0. constructor; auto.
+  - (* Function call *)
+    inversion_clear H2.
     assert ((params, fstmt, fexpr) = (params0, fstmt0, fexpr0)).
     { apply StringMapFacts.MapsTo_fun with F x; auto. }
     inversion H2; subst params0 fstmt0 fexpr0; clear H2.
     apply NM_CallOrInvocation with params fstmt' fexpr'; auto.
-    subst F'. apply StringMapFacts.add_mapsto_iff. auto.
-  - intros. inversion_clear H0. apply StringMap_mapsto_in in m. contradiction.
-  - intros. inversion_clear H1. constructor; auto.
+    + (* Prove that transformed arguments don't contain macro invocations *)
+      subst F''''. apply ExprListNoMacroInvocations_update_ExprNoCallsFromFunctionTableExprList_ExprListNoMacroInvocations; auto.
+      subst F'''. apply ExprListNoMacroInvocations_update_ExprNoCallsFromFunctionTableExprList_ExprListNoMacroInvocations; auto.
+      subst F''. apply ExprListNoMacroInvocations_update_ExprNoCallsFromFunctionTableExprList_ExprListNoMacroInvocations; auto.
+    + (* Prove that the function can actually be found in the tranformed
+         function table *)
+      subst F'''' newdef. apply StringMapFacts.add_mapsto_iff.
+      left. auto.
+    + (* Prove that the transformed function expression does not contain
+         macro invocations *)
+      subst F''''. apply ExprNoMacroInvocations_update_ExprNoCallFromFunctionTable_ExprNoMacroInvocations; auto.
+      apply H1.
+      subst F''. apply ExprNoMacroInvocations_update_ExprNoCallFromFunctionTable_ExprNoMacroInvocations; auto.
+      subst F'. apply ExprNoMacroInvocations_update_ExprNoCallFromFunctionTable_ExprNoMacroInvocations; auto.
+  - (* Macro invocation 
+    (can't happen since we are assuming no macro invocations *)
+    intros. inversion_clear H0. apply StringMap_mapsto_in in m. contradiction.
+  - (* ExprList *)
+    intros. inversion_clear H1. constructor; auto.
 Qed.
 
 
-Lemma TransformArgs_ExprNoMacroInvocationsArgs_e_eq: forall M F es F' es',
-  TransformArgs M F es F' es' ->
-  NoMacroInvocationsArgs es F M ->
+Lemma TransformExprList_ExprExprListNoMacroInvocations_e_eq: forall M F es F' es',
+  TransformExprList M F es F' es' ->
+  ExprListNoMacroInvocations es F M ->
   es = es'.
 Proof.
   intros. induction H; auto.
-  inversion_clear H0. f_equal; auto.
-  eapply TransformExpr_ExprNoMacroInvocations_e_eq; eauto.
+  inversion_clear H0. f_equal;
+    eauto using TransformExpr_ExprNoMacroInvocations_e_eq.
 Qed.
 
 
-Lemma TransformArgs_NoMacroInvocationsArgs_NoMacroInvocationsArgs : forall M F es F' es',
-  TransformArgs M F es F' es' ->
-  NoMacroInvocationsArgs es F M ->
-  NoMacroInvocationsArgs es' F' M.
+Lemma TransformExprList_ExprListNoMacroInvocations_ExprListNoMacroInvocations : forall M F es F' es',
+  TransformExprList M F es F' es' ->
+  ExprListNoMacroInvocations es F M ->
+  ExprListNoMacroInvocations es' F' M.
 Proof.
-  apply (TransformArgs_mut
-    (* TransformExpr *)
-    (fun M F e F' e' (h : TransformExpr M F e F' e') =>
-      ExprNoMacroInvocations e F M ->
-      ExprNoMacroInvocations e' F' M)
-    (* TransformArgs *)
-    (fun M F es F' es' (h : TransformArgs M F es F' es') =>
-      NoMacroInvocationsArgs es F M ->
-      NoMacroInvocationsArgs es' F' M)
-    (* TransformStmt *)
-    (fun M F stmt F' stmt' (h : TransformStmt M F stmt F' stmt') =>
-      True (* TODO: Fix this later once we add more statements *))); intros; auto.
-  - inversion_clear H0. constructor; auto.
-  - inversion_clear H0. constructor; auto.
-  - inversion_clear H1. constructor.
-    +
-      subst F''.
-      apply ExprNoMacroInvocations_update_ExprNoCallFromFunctionTable_ExprNoMacroInvocations;
-        auto.
-    +
-      subst F''.
-      apply ExprNoMacroInvocations_update_ExprNoCallFromFunctionTable_ExprNoMacroInvocations with
-        (F':=F1result) in H3; auto.
-      rewrite <- e in H3. auto.
-  - inversion_clear H0. constructor; auto.
-  - inversion_clear H2. econstructor; auto.
-    + rewrite e. apply StringMapFacts.add_mapsto_iff. left; auto.
-    + apply H1.
-      assert ((params, fstmt, fexpr) = (params0, fstmt0, fexpr0)).
-      { apply StringMapFacts.MapsTo_fun with F x; auto. }
-      inversion_clear H2. auto.
-  - inversion_clear H0. apply StringMap_mapsto_in in m. contradiction.
-  - inversion_clear H1. constructor; auto.
+  intros. induction H.
+  - (* nil *)
+    constructor.
+  - (* cons *)
+    inversion_clear H0. constructor;
+      eauto using TransformExpr_ExprNoMacroInvocations_ExprNoMacroInvocations.
 Qed.
